\documentclass[12pt]{article}
\usepackage[utf8]{inputenc}
\usepackage{amsmath, amssymb, amsthm}
\usepackage{enumitem}
\usepackage{geometry}
\usepackage{fancyhdr}
\DeclareMathOperator{\Tr}{Tr}

% Page setup
\setlength{\headheight}{15pt}
\geometry{letterpaper, margin=1in}
\setlength{\parindent}{0pt}
\setlength{\parskip}{1em}
\pagestyle{fancy}
\fancyhf{}
\fancyhead[L]{\textbf{Sebastian Griego}}  % Replace with your name
\fancyhead[C]{\textbf{ODEs}}  % Replace with your course name
\fancyhead[R]{\textbf{Assignment \#2}}  % Replace with your assignment number
\fancyfoot[C]{\thepage}

\newenvironment{problem}[1]{
    \textbf{Problem #1:}
}{
    \rmfamily \vspace{1em}
}

\newenvironment{solution}{
    \textbf{Solution:}
    
}{
    
    \vspace{2em}
}

\begin{document}

\title{Homework \#2}  % Replace with the homework number
\author{Sebastian Griego}  % Replace with your name
\maketitle

\begin{problem}{1}
Solve
    \[
        \frac{dy}{dx} + 2xy = f(x), \quad y(0) = 2
    \]
    where
    \[
        f(x) = \begin{cases}
            x, & 0 \leq x < 1 \\
            2x, & 1 \leq x < 2 \\
            3x, & 2 \leq x < 3 \\
            0, & x \geq 3
        \end{cases}
    \]
\end{problem}

\begin{solution}
    \[
        \frac{dy}{dx} + 2xy = f(x), \quad y(0) = 2
    \]
    Define the integrating factor:
    \[
        \Phi(x,s) = e^{-\int_{s}^{x} 2t \, dt} = e^{-(x^2 - s^2)}
    \]
    Solution to the ODE:
    \[
    \begin{aligned}
        y(x) &= \Phi(x,0) \cdot y(0) + \int_{0}^{x} \Phi(x,s) \cdot f(s) \, ds \\
        &= 2e^{-x^2} + \int_{0}^{x} e^{-(x^2 - s^2)} \cdot f(s) \, ds
    \end{aligned}
    \]
    Evaluate the integral for each interval of $f(x)$:
    \begin{itemize}
        \item For $0 \leq x < 1$:
        \[
        \begin{aligned}
            \int_{0}^{x} e^{-(x^2 - s^2)} \cdot s \, ds &= \int_{0}^{x} e^{-(x^2 - s^2)} \cdot s \, ds \\
            &= \int_{0}^{x} e^{s^2-x^2} \cdot s \, ds\\
            &= \frac{1}{2}\int e^{u} \, du \quad u = s^2 - x^2\\
            &= \frac{e^u}{2}\\
            &= \frac{e^{s^2 - x^2}}{2} \bigg|_{0}^{x}\\
            &= \frac{e^{x^2 - x^2}}{2} - \frac{e^{0^2 - x^2}}{2}\\
            &= \frac{1-e^{-x^2}}{2}\\
            &= \frac{-e^{-x^2}}{2} + \frac{1}{2}
        \end{aligned}
        \]
        \item For $1 \leq x < 2$:
        \[
        \begin{aligned}
            \int_{0}^{1} e^{-(x^2 - s^2)} \cdot s \, ds + \int_{1}^{x} e^{-(x^2 - s^2)} \cdot 2s \, ds &= \int_{0}^{1} e^{-(x^2 - s^2)} \cdot s \, ds + 2\int_{1}^{x} e^{-(x^2 - s^2)} \cdot s \, ds \\
            &= \frac{e^{s^2 - x^2}}{2} \bigg|_{0}^{1} + 2 \cdot \frac{e^{s^2 - x^2}}{2} \bigg|_{1}^{x}\\
            &= \frac{e^{1-x^2} - e^{-x^2}}{2} + 1 - e^{1-x^2}\\
            &= \frac{-e^{-x^2}}{2} - \frac{e^{1-x^2}}{2} + 1\\
        \end{aligned}
        \]
        \item For $2 \leq x < 3$:
        \[
        \begin{aligned}
            &\int_{0}^{1} e^{-(x^2 - s^2)} \cdot s \, ds + 2\int_{1}^{2} e^{-(x^2 - s^2)} \cdot s \, ds + 3\int_{2}^{x} e^{-(x^2 - s^2)} \cdot s \, ds\\
            &= \frac{e^{1-x^2} - e^{-x^2}}{2} + 2 \cdot \frac{e^{s^2 - x^2}}{2} \bigg|_{1}^{2} + 3 \cdot \frac{e^{s^2 - x^2}}{2} \bigg|_{2}^{x}\\
            &= \frac{e^{1-x^2} - e^{-x^2}}{2} + \frac{2e^{4-x^2} - 2e^{1-x^2}}{2} + \frac{3 - 3e^{4-x^2}}{2}\\
            &= \frac{-e^{-x^2}}{2} - \frac{e^{1-x^2}}{2} - \frac{e^{4-x^2}}{2} + \frac{3}{2}\\
        \end{aligned}
        \]
        \item For $x \geq 3$:
        \[
        \begin{aligned}
            &\int_{0}^{1} e^{-(x^2 - s^2)} \cdot s \, ds + \int_{1}^{2} e^{-(x^2 - s^2)} \cdot 2s \, ds + \int_{2}^{3} e^{-(x^2 - s^2)} \cdot 3s \, ds + \int_{3}^{x} e^{-(x^2 - s^2)} \cdot 0 \, ds\\
            &= \int_{0}^{1} e^{-(x^2 - s^2)} \cdot s \, ds + \int_{1}^{2} e^{-(x^2 - s^2)} \cdot 2s \, ds + \int_{2}^{3} e^{-(x^2 - s^2)} \cdot 3s \, ds\\
            &= \frac{e^{1-x^2} - e^{-x^2}}{2} + \frac{2e^{4-x^2} - 2e^{1-x^2}}{2} + 3 \cdot \frac{e^{s^2 - x^2}}{2} \bigg|_{2}^{3}\\
            &= \frac{e^{1-x^2} - e^{-x^2}}{2} + \frac{2e^{4-x^2} - 2e^{1-x^2}}{2} + \frac{3e^{9 - x^2} - 3e^{4 - x^2}}{2}\\
            &= \frac{-e^{-x^2}}{2} - \frac{e^{1-x^2}}{2} - \frac{e^{4-x^2}}{2} + \frac{3e^{9 - x^2}}{2}\\
        \end{aligned}
        \]
    \end{itemize}
Remember, the solution is
    \[
    y(x) = 2e^{-x^2} + \int_{0}^{x} e^{-(x^2 - s^2)} \cdot f(s) \, ds
    \]
The leading term of all the previous integrals is \(\frac{-e^{-x^2}}{2}\), so adding \(2e^{-x^2}\) to them gives the leading term of the solution, \(\frac{3e^{-x^2}}{2}\). All the other terms stay the same. This gives a final solution of
    \[
    y(x) = \begin{cases}
        \frac{3e^{-x^2}}{2} + \frac{1}{2}, & 0 \leq x < 1 \\
        \frac{3e^{-x^2}}{2} - \frac{e^{1-x^2}}{2} + 1, & 1 \leq x < 2 \\
        \frac{3e^{-x^2}}{2} - \frac{e^{1-x^2}}{2} - \frac{e^{4-x^2}}{2} + \frac{3}{2}, & 2 \leq x < 3 \\
        \frac{3e^{-x^2}}{2} - \frac{e^{1-x^2}}{2} - \frac{e^{4-x^2}}{2} + \frac{3e^{9 - x^2}}{2}, & x \geq 3
    \end{cases}
    \]
\end{solution}

\begin{problem}{2}
    Find the solution of the initial value problem \(\frac{d\vec{x}}{dt} = A\vec{x}, \; \vec{x}(0) = \vec{x_0} \; \) for \(A\) given by
    \[
        A = \begin{pmatrix}
            2 & -1 \\
            -1 & 1
        \end{pmatrix}
    \]
\end{problem}

\begin{solution}
    Start with
    \[
        \frac{d\vec{x}}{dt} = A\vec{x}, \; \vec{x}(0) = \vec{x_0} \;
    \]
    The solution is given by
    \[
        \vec{x}(t) = V\begin{pmatrix}
            e^{\lambda_1 t} & 0 \\
            0 & e^{\lambda_2 t}
        \end{pmatrix}V^{-1}\vec{x_0}
    \]
    Find eigenvalues and eigenvectors of \(A\):
    \[
        \begin{aligned}
            p(\lambda) &= \lambda^2 - \Tr(A)\lambda + \det(A) \\
            &= \lambda^2 - 3\lambda + 1
        \end{aligned}
    \]
    Set \(p(\lambda) = 0\) and solve for \(\lambda\):
    \[
        \begin{aligned}
            \lambda^2 - 3\lambda + 1 &= 0 \\
            \lambda &= \frac{1}{2} \left(3 \pm {(9 - 4 \cdot 1)}^{\frac{1}{2}}\right) \\
            &= \frac{1}{2} \left(3 \pm 5^{\frac{1}{2}}\right) \\
            &= \frac{1}{2} \left(3 \pm \sqrt{5}\right)
        \end{aligned}
    \]
    So, the eigenvalues are \(\lambda_1 = \frac{3}{2} + \frac{\sqrt{5}}{2}\) and \(\lambda_2 = \frac{3}{2} - \frac{\sqrt{5}}{2}\).

    Find the eigenvectors:
    \begin{itemize}
        \item For \(\lambda_1 = \frac{3}{2} + \frac{\sqrt{5}}{2}\):
        \[
            A - \left(\frac{3}{2} + \frac{\sqrt{5}}{2}\right)I = \begin{pmatrix}
                \frac{1}{2} - \frac{\sqrt{5}}{2} & -1 \\
                -1 & -\frac{1}{2} - \frac{\sqrt{5}}{2}
            \end{pmatrix}
        \]
        Set  \((A - \lambda I)\vec{v} = 0\):
        \[
        \begin{pmatrix}
            \frac{1}{2} - \frac{\sqrt{5}}{2} & -1 \\
            -1 & -\frac{1}{2} - \frac{\sqrt{5}}{2}
        \end{pmatrix}
        \begin{pmatrix}
            v_1 \\
            v_2
        \end{pmatrix} = 0
        \]
        This gives
        \[
            -v_1 + \left(-\frac{1}{2} - \frac{\sqrt{5}}{2}\right)v_2 = 0 \implies v_1 = \left(-\frac{1}{2} - \frac{\sqrt{5}}{2}\right)v_2
        \]
        Set \(v_2 = 1\). Then
        \[
            v_1 = \left(-\frac{1}{2} - \frac{\sqrt{5}}{2}\right)
        \]
        So, the eigenvector is
        \[
            \vec{v} = \begin{pmatrix}
                -\frac{1}{2} - \frac{\sqrt{5}}{2} \\
                1
            \end{pmatrix}
        \]
        \item For \(\lambda_2 = \frac{3}{2} - \frac{\sqrt{5}}{2}\):
        \[
            A - \left(\frac{3}{2} - \frac{\sqrt{5}}{2}\right)I = \begin{pmatrix}
                \frac{1}{2} + \frac{\sqrt{5}}{2} & -1 \\
                -1 & -\frac{1}{2} + \frac{\sqrt{5}}{2}
            \end{pmatrix}
        \]
        Set \((A - \lambda I)\vec{v} = 0\):
        \[
        \begin{pmatrix}
            \frac{1}{2} + \frac{\sqrt{5}}{2} & -1 \\
            -1 & -\frac{1}{2} + \frac{\sqrt{5}}{2}
        \end{pmatrix}
        \begin{pmatrix}
            v_1 \\
            v_2
        \end{pmatrix} = 0
        \]
        This gives
        \[
            -v_1 + \left(-\frac{1}{2} + \frac{\sqrt{5}}{2}\right)v_2 = 0 \implies v_1 = \left(-\frac{1}{2} + \frac{\sqrt{5}}{2}\right)v_2
        \]
        Set \(v_2 = 1\). Then
        \[
            v_1 = \left(-\frac{1}{2} + \frac{\sqrt{5}}{2}\right)
        \]
        So, the eigenvector is
        \[
            \vec{v} = \begin{pmatrix}
                -\frac{1}{2} + \frac{\sqrt{5}}{2} \\
                1
            \end{pmatrix}
        \]
    \end{itemize}
    \(V\) is given by
    \[
        V = \begin{pmatrix}
            -\frac{1}{2} - \frac{\sqrt{5}}{2} & -\frac{1}{2} + \frac{\sqrt{5}}{2} \\
            1 & 1
        \end{pmatrix}
    \]
    Find \(V^{-1}\):
        \[
            \begin{aligned}
                V^{-1} &= \frac{1}{\det(V)} \begin{pmatrix}
                    1 & \frac{1}{2} - \frac{\sqrt{5}}{2} \\
                    -1 & -\frac{1}{2} - \frac{\sqrt{5}}{2}
                \end{pmatrix} \\
                &= \frac{-1}{\sqrt{5}} \begin{pmatrix}
                    1 & \frac{1}{2} - \frac{\sqrt{5}}{2} \\
                    -1 & -\frac{1}{2} - \frac{\sqrt{5}}{2}
                \end{pmatrix}\\
            \end{aligned}
    \]
    Final solution:
    \[
        \begin{aligned}
            \vec{x}(t) &= V\Lambda V^{-1}\vec{x_0} \\
            &= \begin{pmatrix}
                -\frac{1}{2} - \frac{\sqrt{5}}{2} & -\frac{1}{2} + \frac{\sqrt{5}}{2} \\
                1 & 1
            \end{pmatrix}
            \begin{pmatrix}
                e^{\left(\frac{3}{2} + \frac{\sqrt{5}}{2}\right)t} & 0 \\
                0 & e^{\left(\frac{3}{2} - \frac{\sqrt{5}}{2}\right)t}
            \end{pmatrix}
            \frac{-1}{\sqrt{5}} \begin{pmatrix}
                1 & \frac{1}{2} - \frac{\sqrt{5}}{2} \\
                -1 & -\frac{1}{2} - \frac{\sqrt{5}}{2}
            \end{pmatrix}\vec{x_0}
        \end{aligned}
    \]
\end{solution}

\begin{problem}{3}
    For the real \(2 \times 2\) matrix \(A\), consider the initial value problem
    \[
        \dot{x} = Ax, \quad x(0) = x_0
    \]
    Show that if \(A = V\Lambda V^{-1}\) where
    \[
        \Lambda = \begin{pmatrix}
            \lambda_1 & 0 \\
            0 & \lambda_2
        \end{pmatrix}
    \]
    then the solution is given by
    \[
        x(t) = V\begin{pmatrix}
            e^{\lambda_1 t} & 0 \\
            0 & e^{\lambda_2 t}
        \end{pmatrix}V^{-1}x_0
    \]
\end{problem}

\begin{solution}
    Start with
    \[
        \frac{d\vec{x}}{dt} = A\vec{x}, \; \vec{x}(0) = \vec{x_0} \;
    \]
    We want to find the eigenvalues and eigenvectors of \(A\) to decompose it into
    \[
        A = V\Lambda V^{-1} = V\begin{pmatrix}
            \lambda_1 & 0 \\
            0 & \lambda_2
        \end{pmatrix}V^{-1}
    \]
    Find eigenvalues and eigenvectors of \(A\):
    \[
        p(\lambda) = \lambda^2 - \Tr(A)\lambda + \det(A)
    \]
    Set \(p(\lambda) = 0\) and solve for \(\lambda\):
    \[
        \begin{aligned}
            p(\lambda) &= \lambda^2 - \Tr(A)\lambda + \det(A) = 0\\
            \lambda &= \frac{1}{2}\left(\Tr(A) \pm \left((\Tr(A))^2 - 4\det(A)\right)^{\frac{1}{2}}\right)
        \end{aligned}
    \]
    Assume \(\lambda_1\) and \(\lambda_2\) are distinct. Decompose \(A\) into
    \[
        \begin{aligned}
            A &= V\Lambda V^{-1} \\
            &= V\begin{pmatrix}
                \lambda_1 & 0 \\
                0 & \lambda_2
            \end{pmatrix}V^{-1}
        \end{aligned}
    \]
    Go back to the differential equation:
    \[
        \begin{aligned}
            \frac{d\vec{x}}{dt} &= A\vec{x} \\
            \frac{d\vec{x}}{dt} &= V\Lambda V^{-1}\vec{x} \\
            V^{-1}\frac{d\vec{x}}{dt} &= \Lambda V^{-1}\vec{x} \\
            \frac{d}{dt}(V^{-1}\vec{x}) &= \Lambda (V^{-1}\vec{x})
        \end{aligned}
    \]
    Let \(\vec{y} = V^{-1}\vec{x}\). Then
    \[
        \begin{aligned}
            \frac{d\vec{y}}{dt} &= \Lambda \vec{y} \\
            \frac{d}{dt} \begin{pmatrix}
                y_1 \\
                y_2
            \end{pmatrix} &= \begin{pmatrix}
                \lambda_1 & 0 \\
                0 & \lambda_2
            \end{pmatrix} \begin{pmatrix}
                y_1 \\
                y_2
            \end{pmatrix}
        \end{aligned}
    \]
    This gives
    \[
        \begin{aligned}
            \frac{dy_1}{dt} &= \lambda_1 y_1 \\
            \frac{dy_2}{dt} &= \lambda_2 y_2
        \end{aligned}
    \]
    Solve each differential equation:
    \[
        \begin{aligned}
            y_1(t) &= y_1(0) \cdot e^{\lambda_1 t} \\
            y_2(t) &= y_2(0) \cdot e^{\lambda_2 t}
        \end{aligned}
    \]
    Decompose this back into matrix form:
    \[
        \vec{y}(t) = \begin{pmatrix}
            e^{\lambda_1 t} & 0 \\
            0 & e^{\lambda_2 t}
        \end{pmatrix} \vec{y}(0)
    \]
    Given \(\vec{y}(t) = V^{-1}\vec{x}\), we have \(\vec{x}(t) = V\vec{y}(t)\):
    \[
        \begin{aligned}
            \vec{x}(t) &= V\vec{y}(t) \\
            &= V\begin{pmatrix}
                e^{\lambda_1 t} & 0 \\
            0 & e^{\lambda_2 t}
        \end{pmatrix}\vec{y}(0) \\
        &= V\begin{pmatrix}
            e^{\lambda_1 t} & 0 \\
            0 & e^{\lambda_2 t}
        \end{pmatrix}V^{-1}\vec{x_0}
        \end{aligned}
    \]
\end{solution}

\begin{problem}{4}
    Show that if \(A = VJV^{-1}\) where
    \[
        J = \begin{pmatrix}
            \lambda & 1 \\
            0 & \lambda
        \end{pmatrix}
    \]
    then the solution is given by
    \[
        x(t) = V\begin{pmatrix}
            e^{\lambda t} & t e^{\lambda t} \\
            0 & e^{\lambda t}
        \end{pmatrix}V^{-1}x_0
    \]
\end{problem}

\begin{solution}
    Start with
    \[
        \frac{d\vec{x}}{dt} = A\vec{x}, \; \vec{x}(0) = \vec{x_0} \;
    \]
    From the previous problem, the eigenvalues are
    \[
    \lambda = \frac{1}{2}\left(\Tr(A) \pm \left((\Tr(A))^2 - 4\det(A)\right)^{\frac{1}{2}}\right)
    \]
    Assume the eigenvalues are equal. Then the matrix \(A\) can be decomposed as
    \[
        A = VJV^{-1}
    \]
    where
    \[
        J = \begin{pmatrix}
            \lambda & 1 \\
            0 & \lambda
        \end{pmatrix}
    \]
    Go back to the differential equation:
    \[
        \begin{aligned}
            \frac{d\vec{x}}{dt} &= A\vec{x} \\
            \frac{d\vec{x}}{dt} &= VJV^{-1}\vec{x} \\
            V^{-1}\frac{d\vec{x}}{dt} &= JV^{-1}\vec{x} \\
            \frac{d}{dt}(V^{-1}\vec{x}) &= J (V^{-1}\vec{x})
        \end{aligned}
    \]
    Let \(\vec{y} = V^{-1}\vec{x}\). Then
    \[
        \begin{aligned}
            \frac{d\vec{y}}{dt} &= J\vec{y} \\
            \frac{d}{dt} \begin{pmatrix}
                y_1 \\
                y_2
            \end{pmatrix} &= \begin{pmatrix}
                \lambda & 1 \\
                0 & \lambda
            \end{pmatrix} \begin{pmatrix}
                y_1 \\
                y_2
            \end{pmatrix}
        \end{aligned}
    \]
    This gives
    \[
        \begin{aligned}
            \frac{dy_1}{dt} &= \lambda y_1 + y_2 \\
            \frac{dy_2}{dt} &= \lambda y_2
        \end{aligned}
    \]
    Solve the second equation:
    \[
        y_2(t) = y_2(0) \cdot e^{\lambda t}
    \]
    Substitute and solve the first equation:
    \[
        \begin{aligned}
            \frac{dy_1}{dt} &= \lambda y_1 + y_2(0) \cdot e^{\lambda t} \\
            y_1(t) &= y_1(0) \cdot e^{\lambda t} + y_2(0) \cdot t e^{\lambda t} \\
        \end{aligned}
    \]
    We get
    \[
        \begin{aligned}
            y_1(t) &= y_1(0) \cdot e^{\lambda t} + y_2(0) \cdot t e^{\lambda t} \\
            y_2(t) &= y_2(0) \cdot e^{\lambda t}\\
        \end{aligned}
    \]
    Decompose this back into matrix form:
    \[
        \begin{aligned}
            \vec{y}(t) &= \begin{pmatrix}
                e^{\lambda t} & t e^{\lambda t} \\
                0 & e^{\lambda t}
            \end{pmatrix} \begin{pmatrix}
                y_1(0) \\
                y_2(0)
            \end{pmatrix}\\
            &= \begin{pmatrix}
                e^{\lambda t} & t e^{\lambda t} \\
                0 & e^{\lambda t}
            \end{pmatrix} \vec{y}(0)
        \end{aligned}
    \]
    Given \(\vec{y}(t) = V^{-1}\vec{x}\), we have \(\vec{x}(t) = V\vec{y}(t)\):
    \[
        \begin{aligned}
            \vec{x}(t) &= V\vec{y}(t) \\
            &= V\begin{pmatrix}
                e^{\lambda t} & t e^{\lambda t} \\
                0 & e^{\lambda t}
            \end{pmatrix}\vec{y}(0) \\
            &= V\begin{pmatrix}
                e^{\lambda t} & t e^{\lambda t} \\
                0 & e^{\lambda t}
            \end{pmatrix}V^{-1}\vec{x_0}
        \end{aligned}
    \]
\end{solution}



\end{document}